Start work on relatedness interface

theories/Monad/Free_Relation.v
@@ -34,6 +34,7 @@ From Em Require Import
   Related.Interface
   Prefix.
 From Em Require Free_Shallow Free_Deep.
+Import (hints) Free_Shallow Free_Deep.
 
 Module S := Free_Shallow.
 Module D := Free_Deep.
@@ -42,27 +43,42 @@ Import Pred Pred.notations Pred.Sub Pred.proofmode world.notations.
 
 #[local] Set Implicit Arguments.
 
-Inductive RFree (DA : OType) (SA : Type) (RA : Rel DA SA) : Rel (D.Free DA) (S.Free SA) :=
-  | ret : forall w da sa ass, RA w da sa ass -> @RFree DA SA RA w (D.Ret da) (S.Ret sa) ass
+Import logicalrelation.
+
+Inductive RawFree (DA : OType) (SA : Type) (RA : Rel DA SA) : RawRel (D.Free DA) (S.Free SA) :=
+  | ret : forall w da sa ass, RSat RA da sa ass -> @RawFree DA SA RA w (D.Ret da) (S.Ret sa) ass
   | pickk w α (dk : D.Free DA (w ، α)) (sk : Ty -> S.Free SA) ass
-          (rk : forall st, @RFree DA SA RA (w ، α) dk (sk st) (env.snoc ass α st))
-    : @RFree DA SA RA w (D.Pickk α dk) (S.Pickk sk) ass.
+          (rk : forall st, @RawFree DA SA RA (w ، α) dk (sk st) (env.snoc ass α st))
+    : @RawFree DA SA RA w (D.Pickk α dk) (S.Pickk sk) ass.
 
 Goal False. match type of @pickk with ?t => let t' := eval cbv [RTy] in t in idtac t' end. Abort.
 
-Definition rwp {DA SA} (RA : Rel DA SA) : Rel (D.Free DA ⇢ Box Prefix (DA ⇢ Pred) ⇢ Pred) (S.Free SA -> (SA -> Prop) -> Prop).
-apply RArr. apply RFree. apply RA. apply RArr. apply RBox. apply RArr. apply RA. all: apply RPred. Defined.
+Definition RFree (DA : OType) (SA : Type) (RA : Rel DA SA) : Rel (D.Free DA) (S.Free SA) :=
+  MkRel (RawFree RA).
 
-Lemma wlps_are_related : Prop.
-  eapply rwp. exact RTy. apply D.wp_free. apply S.wp_free. apply env.nil. Abort.
-(* Generalizing *)
-Lemma wlps_are_related : forall w ass, rwp RTy (@D.wp_free OTy w) (S.wp_free (A:=Ty)) ass.
-  intros w ass. unfold rwp.
-  intros dm sm rm. induction rm; cbn; intros dpost spost rpost.
-  - apply rpost. apply inst_refl. auto.
-  - unfold RPred. unfold wp. setoid_rewrite inst_step. split.
-    + intros. destruct H0. destruct env.view. exists v. specialize rk with v. destruct H0. unfold RArr, RBox in *.
-      specialize (H v (_4 dpost step) spost). subst. eapply H in H1. auto. intros w' θ ass' eq.
-      unfold _4. apply rpost. rewrite inst_trans inst_step eq. now simpl.
-    + intros. destruct H0. exists (env.snoc ass α x). cbn. split. auto. eapply H; eauto. intros w' θ ass' eq. apply rpost. rewrite inst_trans inst_step eq. now simpl.
+Definition rwp {DA SA} (RA : Rel DA SA) : Rel (D.Free DA ⇢ Box Prefix (DA ⇢ Pred) ⇢ Pred) (S.Free SA -> (SA -> Prop) -> Prop).
+apply RImpl. apply RFree. apply RA. apply RImpl. apply RBox. apply RImpl. apply RA. all: apply RPred. Defined.
+
+#[export] Instance rpure_free : RPure RFree.
+Proof.
+  intros DA SA RA.
+  intros w.
+  cbn.
+  constructor.
+  intros ι _ da sa ra.
+  now constructor.
 Qed.
+
+(* Lemma wlps_are_related : Prop. *)
+(*   eapply rwp. exact RTy. apply D.wp_free. apply S.wp_free. apply env.nil. Abort. *)
+(* (* Generalizing *) *)
+(* Lemma wlps_are_related : forall w ass, rwp RTy (@D.wp_free OTy w) (S.wp_free (A:=Ty)) ass. *)
+(*   intros w ass. unfold rwp. *)
+(*   intros dm sm rm. induction rm; cbn; intros dpost spost rpost. *)
+(*   - apply rpost. apply inst_refl. auto. *)
+(*   - unfold RPred. unfold wp. setoid_rewrite inst_step. split. *)
+(*     + intros. destruct H0. destruct env.view. exists v. specialize rk with v. destruct H0. unfold RArr, RBox in *. *)
+(*       specialize (H v (_4 dpost step) spost). subst. eapply H in H1. auto. intros w' θ ass' eq. *)
+(*       unfold _4. apply rpost. rewrite inst_trans inst_step eq. now simpl. *)
+(*     + intros. destruct H0. exists (env.snoc ass α x). cbn. split. auto. eapply H; eauto. intros w' θ ass' eq. apply rpost. rewrite inst_trans inst_step eq. now simpl. *)
+(* Qed. *)
