theories/Related/Interface.v
@@ -29,7 +29,8 @@
 Require Import Coq.Classes.RelationClasses.
 From iris Require Import proofmode.tactics.
 From Em Require Import BaseLogic Prefix Spec.
-From Em Require Monad.Interface Shallow.Interface.
+From Em Require Free_Deep Free_Shallow
+  Monad.Interface Shallow.Interface.
 
 Module S := Shallow.Interface.
 Module D := Monad.Interface.
@@ -38,22 +39,461 @@ Import Pred Pred.notations Pred.Sub Pred.proofmode world.notations.
 
 #[local] Set Implicit Arguments.
 
-Definition Rel (DA : OType) (SA : Type) : Type :=
-  forall (w : World) , DA w -> SA -> Pred w.
+Declare Scope rel_scope.
+Delimit Scope rel_scope with R.
 
-Definition RTy : Rel OTy Ty :=
-  fun w (T : OTy w) (t : Ty) (ass : Assignment w) =>
-    inst T ass = t.
+Module logicalrelation.
 
-(* For functions/impl: related inputs go to related outputs *)
-Definition RArr {DA SA DB SB} (RA : Rel DA SA) (RB : Rel DB SB) : Rel (DA ⇢ DB) (SA -> SB) :=
-  fun w df sf ass => forall (da : DA w) (sa : SA)
-                            (ra : RA w da sa ass),
-      RB w (df da) (sf sa) ass.
+  Definition RawRel (DA : OType) (SA : Type) : Type :=
+    forall (w : World), DA w -> SA -> Pred w.
+  Class Rel (DA : OType) (SA : Type) : Type :=
+    MkRel { RSat : forall (w : World), DA w -> SA -> Pred w }.
 
-Definition RBox {DA SA} (RA : Rel DA SA) : Rel (Box Prefix DA) SA :=
-  fun (w : World) (bda : (◻⁺DA)%W w) (sa : SA) =>
-         PBox (λ (w' : World) (θ : w ⊑⁺ w'), RA w' (bda w' θ) sa).
+  Bind Scope rel_scope with Rel.
+  #[global] Arguments MkRel [DA SA] &.
+  #[global] Arguments RSat {_ _} _ {w} ι _ _.
 
-Definition RPred : Rel Pred Prop.
-unfold Rel, Pred. intros w DP SP ass. refine (DP ass <-> SP). Defined.
+  Definition RValid {DA SA} (RA : Rel DA SA) (d : Valid DA) (s : SA) : Prop :=
+    forall (w : World), (⊢ @RSat DA SA RA w (d w) s).
+  #[local] Notation "ℛ⟦ R ⟧@{ ι }" := (RSat R%R ι) (format "ℛ⟦ R ⟧@{ ι }") .
+  #[local] Notation "ℛ⟦ R ⟧" := (RValid R%R) (format "ℛ⟦ R ⟧").
+
+  (* This instance can be used for any (first-class) symbolic data that can be
+       instantiated with a valuation, i.e. symbolic terms, stores, heaps etc. *)
+  Definition RInst AT A {instA : Inst AT A} : Rel AT A :=
+    MkRel (fun w d s ι => s = inst d ι)%P.
+  Arguments RInst _ _ {_}.
+
+  #[export] Instance RBox {DA SA} (RA : Rel DA SA) : Rel (Box Prefix DA) SA :=
+    MkRel (fun (w : World) (bda : Box Prefix DA w) (sa : SA) =>
+             PBox (fun (w' : World) (θ : w ⊑⁺ w') => RSat RA (bda w' θ) sa)).
+
+
+  (* For functions/impl: related inputs go to related outputs *)
+  #[export] Instance RImpl {DA SA DB SB} (RA : Rel DA SA) (RB : Rel DB SB) :
+    Rel (DA ⇢ DB) (SA -> SB) :=
+    MkRel
+      (fun w df sf =>
+         ∀ (da : DA w) (sa : SA),
+           RSat RA da sa → RSat RB (df da) (sf sa))%I.
+
+  (* #[export] Instance RForall {𝑲} *)
+  (*   {AT : forall K : 𝑲, TYPE} {A : forall K : 𝑲, Type} *)
+  (*   (RA : forall K, Rel (AT K) (A K)) : *)
+  (*   Rel (@Forall 𝑲 AT) (forall K : 𝑲, A K) := *)
+  (*   MkRel (fun w ι fs fc => *)
+  (*            forall K : 𝑲, *)
+  (*              ℛ⟦RA K⟧@{ι} (fs K) (fc K)). *)
+
+  #[export] Instance RTy : Rel OTy Ty :=
+    RInst OTy Ty.
+
+  #[export] Instance RUnit : Rel Unit unit := RInst Unit unit.
+
+  #[export] Instance RConst A : Rel (Const A) A := RInst (Const A) A.
+
+  (* #[export] Instance RProd `(RA : Rel AT A, RB : Rel BT B) : *)
+  (*   Rel (WProd AT BT) (A * B)%type := *)
+  (*   MkRel (fun w ι '(ta,tb) '(va,vb) => *)
+  (*            ℛ⟦RA⟧@{ι} ta va /\ ℛ⟦RB⟧@{ι} tb vb). *)
+
+  Module Import notations.
+    Open Scope rel_scope.
+    (* Notation "ℛ⟦ R ⟧@{ ι }" := (RSat R%R ι) (format "ℛ⟦ R ⟧@{ ι }"). *)
+    Notation "ℛ⟦ R ⟧" := (RValid R%R) (format "ℛ⟦ R ⟧").
+    Notation "A ↣ B" :=
+      (RImpl A%R B%R)
+        (at level 99, B at level 200, right associativity)
+        : rel_scope.
+    Notation "□ A"    := (RBox A%R) : rel_scope.
+    (* Notation "'∀' x .. y , R " := *)
+    (*   (RForall (fun x => .. (RForall (fun y => R)) ..)) *)
+    (*     (at level 200, x binder, y binder, right associativity, *)
+    (*       format "'[  ' '[  ' ∀  x  ..  y ']' ,  '/' R ']'") *)
+    (*     : rel_scope. *)
+  End notations.
+
+  #[export] Instance RPred : Rel Pred Prop :=
+    MkRel (fun w DP SP ι => DP ι <-> SP ).
+
+  Section MonadClasses.
+
+    Context (DM : OType → OType) (SM : Type -> Type)
+      (RM : forall {DA SA} (RA : Rel DA SA), Rel (DM DA) (SM SA)).
+
+    Class RPure `{D.Pure DM, MRet SM} : Type :=
+      rpure DA SA (RA : Rel DA SA) :
+        ℛ⟦RA ↣ RM RA⟧ D.pure (mret).
+
+  End MonadClasses.
+
+End logicalrelation.
+
+
+(*     Class RBind (DM : OType → OType) (SM : Type -> Type) `{D.Pure DM, MRet SM} *)
+(*     (RM : forall DA SA (RA : Rel DA SA), Rel (DM DA) (SM SA)) *)
+(*     (M : OType → OType) : Type := *)
+(*     bind : ∀ A B, ⊧ M A ⇢ Box Θ (A ⇢ M B) ⇢ M B. *)
+(* #[global] Arguments bind {Θ M _ A B} [w]. *)
+(* Class Fail (M : OType → OType) : Type := *)
+(*   fail : ∀ A, ⊧ M A. *)
+(* #[global] Arguments fail {M _ A w}. *)
+
+(* Module MonadNotations. *)
+(*   Notation "' x <- ma ;; mb" := *)
+(*     (bind ma (fun _ _ x => mb)) *)
+(*       (at level 80, x pattern, ma at next level, mb at level 200, right associativity, *)
+(*         format "' x  <-  ma  ;;  mb"). *)
+(*   Notation "x <- ma ;; mb" := *)
+(*     (bind ma (fun _ _ x => mb)) *)
+(*       (at level 80, ma at next level, mb at level 200, right associativity). *)
+
+(*   Existing Class sub. *)
+(*   #[export] Existing Instance trans. *)
+(*   #[export] Hint Mode sub - + - : typeclass_instances. *)
+(* End MonadNotations. *)
+
+(* Import Pred Pred.Sub. *)
+
+
+(* Class TypeCheckM (M : OType -> OType) : Type := *)
+(*   { equals : ⊧ OTy ⇢ OTy ⇢ M Unit; *)
+(*     pick   : ⊧ M OTy; *)
+(*   }. *)
+(* #[global] Arguments fail {_ _ _ w}. *)
+(* #[global] Arguments pick {_ _ w}. *)
+
+(* Class WeakestPre (Θ : SUB) (M : OType -> OType) : Type := *)
+(*   WP [A] : ⊧ M A ⇢ Box Θ (A ⇢ Pred) ⇢ Pred. *)
+(* Class WeakestLiberalPre (Θ : SUB) (M : OType -> OType) : Type := *)
+(*   WLP [A] : ⊧ M A ⇢ Box Θ (A ⇢ Pred) ⇢ Pred. *)
+
+(* Class AxiomaticSemantics *)
+(*   Θ {reflΘ : Refl Θ} {stepΘ : Step Θ} {transΘ : Trans Θ } {reflTransΘ : ReflTrans Θ} *)
+(*     {lkreflΘ : LkRefl Θ} {lkStepθ : LkStep Θ} {lktransΘ : LkTrans Θ} *)
+(*   M {pureM : Pure M} {bindM : Bind Θ M} {failM : Fail M} {tcM : TypeCheckM M} *)
+(*     {wpM : WeakestPre Θ M} {wlpM : WeakestLiberalPre Θ M} : Type := *)
+
+(*   { ax_wp_pure [A w] (a : A w) (Q : ◻(A ⇢ Pred) w) : *)
+(*       WP (pure a) Q ⊣⊢ₚ Q _ refl a; *)
+(*     ax_wp_bind [A B w0] (m : M A w0) (f : ◻(A ⇢ M B) w0) (Q : ◻(B ⇢ Pred) w0) : *)
+(*       WP (bind m f) Q ⊣⊢ₚ WP m (fun _ θ1 a => WP (f _ θ1 a) (fun _ θ2 => Q _ (θ1⊙θ2))); *)
+(*     ax_wp_equals [w] (σ τ : OTy w) (Q : ◻(Unit ⇢ Pred) w) : *)
+(*       WP (equals σ τ) Q ⊣⊢ₚ σ =ₚ τ /\ₚ Q _ refl tt; *)
+(*     ax_wp_pick [w] (Q : ◻(OTy ⇢ Pred) w) : *)
+(*       let α := world.fresh w in *)
+(*       WP pick Q ⊣⊢ₚ Sub.wp step (Q (w ، α) step (oty.evar world.in_zero)); *)
+(*     ax_wp_fail [A w] (Q : ◻(A ⇢ Pred) w) : *)
+(*       WP fail Q ⊣⊢ₚ ⊥ₚ; *)
+(*     ax_wp_mono [A w] (m : M A w) (P Q : ◻(A ⇢ Pred) w) : *)
+(*       ◼(fun _ θ1 => ∀ a, P _ θ1 a -∗ Q _ θ1 a) ⊢ *)
+(*       (WP m P -∗ WP m Q); *)
+
+(*     ax_wlp_pure [A w] (a : A w) (Q : ◻(A ⇢ Pred) w) : *)
+(*       WLP (pure a) Q ⊣⊢ₚ Q _ refl a; *)
+(*     ax_wlp_bind [A B w0] (m : M A w0) (f : ◻(A ⇢ M B) w0) (Q : ◻(B ⇢ Pred) w0) : *)
+(*       WLP (bind m f) Q ⊣⊢ₚ WLP m (fun w1 θ1 a => WLP (f _ θ1 a) (fun _ θ2 => Q _ (trans θ1 θ2))); *)
+(*     ax_wlp_equals [w] (σ τ : OTy w) (Q : ◻(Unit ⇢ Pred) w) : *)
+(*       WLP (equals σ τ) Q ⊣⊢ₚ σ =ₚ τ ->ₚ Q _ refl tt; *)
+(*     ax_wlp_pick [w] (Q : ◻(OTy ⇢ Pred) w) : *)
+(*       let α := world.fresh w in *)
+(*       WLP pick Q ⊣⊢ₚ Sub.wlp step (Q (w ، α) step (oty.evar world.in_zero)); *)
+(*     ax_wlp_fail [A w] (Q : ◻(A ⇢ Pred) w) : *)
+(*       WLP fail Q ⊣⊢ₚ ⊤ₚ; *)
+(*     ax_wlp_mono [A w] (m : M A w) (P Q : ◻(A ⇢ Pred) w) : *)
+(*       ◼(fun _ θ1 => ∀ a, P _ θ1 a -∗ Q _ θ1 a) ⊢ *)
+(*       (WLP m P -∗ WLP m Q); *)
+
+(*     ax_wp_impl [A w] (m : M A w) (P : ◻(A ⇢ Pred) w) (Q : Pred w) : *)
+(*       (WP m P ->ₚ Q) ⊣⊢ₚ WLP m (fun w1 θ1 a1 => P w1 θ1 a1 ->ₚ Q[θ1]); *)
+(*   }. *)
+(* #[global] Arguments AxiomaticSemantics Θ {_ _ _ _ _ _ _} _ {_ _ _ _ _ _}. *)
+
+
+(* (* Alternative rule for pick which substitutes the last variable away *)
+(*  as discussed in the papter. *) *)
+(* Lemma ax_wp_pick_substitute `{AxiomaticSemantics Θ M, Thick Θ} {lkThickΘ : LkThick Θ} *)
+(*   [w] (Q : ◻(OTy ⇢ Pred) w) : *)
+(*   WP pick Q ⊣⊢ₚ *)
+(*     let α := world.fresh w in *)
+(*     (∃ₚ τ : OTy w, (Q (w ، α) step (oty.evar world.in_zero))[thick α (αIn := world.in_zero) τ]). *)
+(* Proof. *)
+(*   rewrite ax_wp_pick; cbn. constructor; intros ι. *)
+(*   unfold Sub.wp; pred_unfold. split. *)
+(*   - intros (ι' & Heq & HQ). destruct (env.view ι') as [ι' τ]. *)
+(*     erewrite inst_step_snoc in Heq. subst. *)
+(*     exists (lift τ). now rewrite inst_thick inst_lift. *)
+(*   - intros (τ & HQ). rewrite inst_thick in HQ. *)
+(*     exists (env.snoc ι _ (inst τ ι)). *)
+(*     now rewrite inst_step_snoc. *)
+(* Qed. *)
+
+(* Class TypeCheckLogicM *)
+(*   Θ {reflΘ : Refl Θ} {stepΘ : Step Θ} {transΘ : Trans Θ } *)
+(*     {lkreflΘ : LkRefl Θ} {lkStepθ : LkStep Θ} *)
+(*   M {pureM : Pure M} {bindM : Bind Θ M} {failM : Fail M} {tcM : TypeCheckM M} *)
+(*     {wpM : WeakestPre Θ M} {wlpM : WeakestLiberalPre Θ M} : Type := *)
+
+(*   { wp_pure [A] {subA : Subst A} *)
+(*       [w] (a : A w) (Q : ◻(A ⇢ Pred) w) : *)
+(*       Q _ refl a ⊢ₚ WP (pure a) Q; *)
+(*     wp_bind [A B w0] (m : M A w0) (f : ◻(A ⇢ M B) w0) (Q : ◻(B ⇢ Pred) w0) : *)
+(*       WP m (fun w1 θ1 a => WP (f _ θ1 a) (fun _ θ2 => Q _ (trans θ1 θ2))) ⊢ₚ WP (bind m f) Q; *)
+(*     wp_equals [w] (σ τ : OTy w) (Q : ◻(Unit ⇢ Pred) w) : *)
+(*       σ =ₚ τ /\ₚ ◼(fun _ θ => Q _ θ tt) ⊢ₚ WP (equals σ τ) Q; *)
+(*     wp_pick [w] [Q : ◻(OTy ⇢ Pred) w] (τ : Ty) : *)
+(*       ◼(fun _ θ => ∀ₚ τ', lift τ =ₚ τ' ->ₚ Q _ θ τ') ⊢ₚ WP pick Q; *)
+(*     wp_fail [A w] (Q : ◻(A ⇢ Pred) w) : *)
+(*       ⊥ₚ ⊢ₚ WP fail Q; *)
+(*     wp_mono [A w] (m : M A w) (P Q : ◻(A ⇢ Pred) w) : *)
+(*       ◼(fun _ θ => ∀ₚ a, P _ θ a -∗ Q _ θ a)%I ⊢ₚ *)
+(*       (WP m P -∗ WP m Q)%I; *)
+
+(*     wlp_pure [A] {subA : Subst A} *)
+(*       [w] (a : A w) (Q : ◻(A ⇢ Pred) w) : *)
+(*       Q _ refl a ⊢ₚ WLP (pure a) Q; *)
+(*     wlp_bind [A B w0] (m : M A w0) (f : ◻(A ⇢ M B) w0) (Q : ◻(B ⇢ Pred) w0) : *)
+(*       WLP m (fun w1 θ1 a => WLP (f _ θ1 a) (fun _ θ2 => Q _ (trans θ1 θ2))) ⊢ₚ WLP (bind m f) Q; *)
+(*     wlp_equals [w] (σ τ : OTy w) (Q : ◻(Unit ⇢ Pred) w) : *)
+(*       σ =ₚ τ ->ₚ ◼(fun _ θ => Q _ θ tt) ⊢ₚ WLP (equals σ τ) Q; *)
+(*     wlp_pick [w] (Q : ◻(OTy ⇢ Pred) w) : *)
+(*       ◼(fun _ θ => ∀ₚ τ, Q _ θ τ) ⊢ₚ WLP pick Q; *)
+(*     wlp_fail [A w] (Q : ◻(A ⇢ Pred) w) : *)
+(*       ⊤ₚ ⊢ₚ WLP fail Q; *)
+(*     wlp_mono [A w] (m : M A w) (P Q : ◻(A ⇢ Pred) w) : *)
+(*       ◼(fun _ θ => ∀ₚ a, P _ θ a -∗ Q _ θ a)%I ⊢ₚ *)
+(*       (WLP m P -∗ WLP m Q)%I; *)
+
+(*     wp_impl [A w] (m : M A w) (P : ◻(A ⇢ Pred) w) (Q : Pred w) : *)
+(*       WLP m (fun w1 θ1 a1 => P w1 θ1 a1 ->ₚ Q[θ1]) ⊢ₚ (WP m P ->ₚ Q); *)
+
+(*   }. *)
+(* #[global] Arguments TypeCheckLogicM Θ {_ _ _ _ _} _ {_ _ _ _ _ _}. *)
+
+(* #[export] Instance axiomatic_tcmlogic `{AxiomaticSemantics Θ M} : *)
+(*   TypeCheckLogicM Θ M. *)
+(* Proof. *)
+(*   constructor; intros. *)
+(*   - now rewrite ax_wp_pure. *)
+(*   - now rewrite ax_wp_bind. *)
+(*   - rewrite ax_wp_equals. iIntros "[#Heq >HQ]". now iSplit. *)
+(*   - rewrite ax_wp_pick. rewrite <- (Sub.intro_wp_step τ). *)
+(*     iIntros "#H !> #Heq". iMod "H". *)
+(*     iSpecialize ("H" $! (oty.evar world.in_zero) with "Heq"). *)
+(*     now rewrite trans_refl_r. *)
+(*   - now rewrite ax_wp_fail. *)
+(*   - apply ax_wp_mono. *)
+(*   - now rewrite ax_wlp_pure. *)
+(*   - now rewrite ax_wlp_bind. *)
+(*   - rewrite ax_wlp_equals. iIntros "#HQ #Heq". *)
+(*     iSpecialize ("HQ" with "Heq"). now iMod "HQ". *)
+(*   - rewrite ax_wlp_pick. iIntros "#HQ !>". iMod "HQ". *)
+(*     iSpecialize ("HQ" $! (oty.evar world.in_zero)). *)
+(*     now rewrite trans_refl_r. *)
+(*   - now rewrite ax_wlp_fail. *)
+(*   - apply ax_wlp_mono. *)
+(*   - now rewrite ax_wp_impl. *)
+(* Qed. *)
+
+(* Lemma wp_mono' `{TypeCheckLogicM Θ M} {A w} (m : M A w) (P Q : ◻(A ⇢ Pred) w) : *)
+(*   (WP m P -∗ ◼(fun _ θ1 => ∀ₚ a1, P _ θ1 a1 -∗ Q _ θ1 a1) -∗ WP m Q)%P. *)
+(* Proof. iIntros "WP PQ". iRevert "WP". now rewrite -wp_mono. Qed. *)
+
+(* Lemma wlp_mono' `{TypeCheckLogicM Θ M} {A w} (m : M A w) (P Q : ◻(A ⇢ Pred) w) : *)
+(*   (WLP m P -∗ ◼(fun _ θ1 => ∀ₚ a1, P _ θ1 a1 -∗ Q _ θ1 a1) -∗ WLP m Q)%P. *)
+(* Proof. iIntros "WP PQ". iRevert "WP". now rewrite -wlp_mono. Qed. *)
+
+(* Definition wp_diamond {Θ : SUB} {A} : *)
+(*   ⊧ Diamond Θ A ⇢ ◻(A ⇢ Pred) ⇢ Pred := *)
+(*   fun w '(existT w1 (θ, a)) Q => Sub.wp θ (Q w1 θ a). *)
+
+(* Definition wlp_diamond {Θ : SUB} {A} : *)
+(*   ⊧ Diamond Θ A ⇢ ◻(A ⇢ Pred) ⇢ Pred := *)
+(*   fun w '(existT w1 (θ, a)) Q => Sub.wlp θ (Q w1 θ a). *)
+
+(* Definition wp_option {A w1 w2} : *)
+(*   Option A w1 -> (A w1 -> Pred w2) -> Pred w2 := *)
+(*   fun o Q => *)
+(*     match o with *)
+(*     | Some a => Q a *)
+(*     | None => ⊥ₚ *)
+(*     end%P. *)
+
+(* Definition wlp_option {A w1 w2} : *)
+(*   Option A w1 -> (A w1 -> Pred w2) -> Pred w2 := *)
+(*   fun o Q => *)
+(*     match o with *)
+(*     | Some a => Q a *)
+(*     | None => ⊤ₚ *)
+(*     end%P. *)
+
+(* Definition Solved (Θ : SUB) (A : OType) : OType := Option (Diamond Θ A). *)
+(* Definition Prenex (A : OType) : OType := Solved Prefix (List (OTy * OTy) * A). *)
+
+(* Section Solved. *)
+
+(*   #[export] Instance wp_solved {Θ : SUB} : WeakestPre Θ (Solved Θ) := *)
+(*     fun A w m Q => wp_option m (fun d => wp_diamond d Q). *)
+(*   #[global] Arguments wp_solved {Θ} {A}%indexed_scope [w] _ _%B _. *)
+(*   #[export] Instance wlp_solved {Θ : SUB} : WeakestLiberalPre Θ (Solved Θ) := *)
+(*     fun A w m Q => wlp_option m (fun d => wlp_diamond d Q). *)
+(*   #[global] Arguments wlp_solved {Θ} {A}%indexed_scope [w] _ _%B _. *)
+
+(*   #[global] Instance params_wp_solved : Params (@wp_solved) 3 := {}. *)
+(*   #[export] Instance proper_wp_solved_bientails {Θ A w} : *)
+(*     Proper *)
+(*       (pointwise_relation _ *)
+(*          (forall_relation *)
+(*             (fun _ => pointwise_relation _ *)
+(*                         (pointwise_relation _ (⊣⊢ₚ))) ==> (⊣⊢ₚ))) *)
+(*       (@wp_solved Θ A w). *)
+(*   Proof. *)
+(*     intros d p q pq. destruct d as [(w1 & r01 & a)|]; cbn; [|easy]. *)
+(*     apply Sub.proper_wp_bientails. apply pq. *)
+(*   Qed. *)
+
+(*   #[export] Instance proper_wp_solved_entails {Θ A w} : *)
+(*     Proper *)
+(*       (pointwise_relation _ *)
+(*          (forall_relation *)
+(*             (fun _ => pointwise_relation _ *)
+(*                         (pointwise_relation _ entails)) ==> entails)) *)
+(*       (@wp_solved Θ A w). *)
+(*   Proof. *)
+(*     intros d p q pq. destruct d as [(w1 & r01 & a)|]; cbn; [|easy]. *)
+(*     apply Sub.proper_wp_entails. apply pq. *)
+(*   Qed. *)
+
+(*   Lemma wp_solved_frame {Θ A w} (m : Solved Θ A w) *)
+(*     (P : ◻(A ⇢ Pred) w) (Q : Pred w) : *)
+(*     WP m P /\ₚ Q ⊣⊢ₚ WP m (fun w1 θ1 a1 => P w1 θ1 a1 /\ₚ subst Q θ1). *)
+(*   Proof. *)
+(*     destruct m as [(w1 & θ1 & a1)|]; cbn. *)
+(*     - now rewrite Sub.and_wp_l. *)
+(*     - now rewrite bi.False_and. *)
+(*   Qed. *)
+
+(*   #[export] Instance pure_solved {Θ} {reflΘ : Refl Θ} : *)
+(*     Pure (Solved Θ) := *)
+(*     fun A w a => Some (existT w (refl, a)). *)
+
+(*   #[export] Instance bind_solved {Θ} {transΘ : Trans Θ} : *)
+(*     Bind Θ (Solved Θ) := *)
+(*     fun A B w m f => *)
+(*       option.bind m *)
+(*         (fun '(existT w1 (θ1,a1)) => *)
+(*            option.bind (f w1 θ1 a1) *)
+(*              (fun '(existT w2 (θ2,b2)) => *)
+(*                 Some (existT w2 (trans θ1 θ2, b2)))). *)
+
+(*   #[export] Instance fail_solved {Θ} : Fail (Solved Θ) := *)
+(*     fun A w => None. *)
+
+(*   Lemma wp_solved_pure {Θ} {reflΘ : Refl Θ} {lkreflΘ : LkRefl Θ} *)
+(*     {A w0} (a : A w0) (Q : ◻(A ⇢ Pred) w0) : *)
+(*     wp_solved (pure (M := Solved Θ) a) Q ⊣⊢ₚ Q _ refl a. *)
+(*   Proof. cbn. now rewrite Sub.wp_refl. Qed. *)
+
+(*   Lemma wp_solved_bind {Θ} {transΘ : Trans Θ} {lkTransΘ : LkTrans Θ} *)
+(*     {A B w0} (m : Solved Θ A w0) (f : ◻(A ⇢ Solved Θ B) w0) *)
+(*     (Q : ◻(B  ⇢ Pred) w0) : *)
+(*     WP (bind m f) Q ⊣⊢ₚ WP m (fun w1 ζ1 a1 => WP (f w1 ζ1 a1) (_4 Q ζ1)). *)
+(*   Proof. *)
+(*     destruct m as [(w1 & r01 & a)|]; cbn; [|reflexivity]. *)
+(*     destruct (f w1 r01 a) as [(w2 & r12 & b2)|]; cbn; *)
+(*       now rewrite ?Sub.wp_trans ?Sub.wp_false. *)
+(*   Qed. *)
+
+(* End Solved. *)
+
+(* #[export] Instance instpred_diamond {Θ A} `{ipA : InstPred A} : *)
+(*   InstPred (Diamond Θ A) := *)
+(*   fun w m => wp_diamond m (fun _ _ a => instpred a). *)
+(* #[export] Instance instpred_solved {Θ A} `{ipA : InstPred A} : *)
+(*   InstPred (Solved Θ A) := *)
+(*   fun w m => WP m (fun _ _ a => instpred a). *)
+
+(* Definition solved_hmap `{HMap Θ1 Θ2} {A} : ⊧ Solved Θ1 A ⇢ Solved Θ2 A := *)
+(*   fun w => option.map (fun '(existT w (θ, a)) => existT w (hmap θ, a)). *)
+
+(* Lemma instpred_solved_hmap `{LkHMap Θ1 Θ2} {A} `{ipA : InstPred A} *)
+(*   {w} (m : Solved Θ1 A w) : *)
+(*   instpred (solved_hmap m) ⊣⊢ₚ instpred m. *)
+(* Proof. destruct m as [(w' & θ & a)|]; cbn; now rewrite ?Sub.wp_hmap. Qed. *)
+
+(* (* Create HintDb wpeq. *) *)
+(* (* #[export] Hint Rewrite *) *)
+(* (*   (@subst_eq OEnv _ _ _ _) *) *)
+(* (*   (@subst_eq OTy _ _ _ _) *) *)
+(* (*   (@subst_trans OEnv _ _) *) *)
+(* (*   (@subst_trans OTy _ _) *) *)
+(* (*   @subst_lift *) *)
+(* (*   @lift_insert *) *)
+(* (*   : wpeq. *) *)
+
+(* Ltac wpeq := *)
+(*   progress *)
+(*     (try done; *)
+(*      try progress cbn; *)
+(*      (* Unfortunately, autorewrite and rewrite strategy blow up with some long *)
+(*         typeclass searches. Simply use rewrite for now. *) *)
+(*      rewrite ?(@subst_eq OEnv _ _ _ _) *)
+(*        ?(@subst_eq OTy _ _ _ _) *)
+(*        ?(@subst_trans OEnv _ _) *)
+(*        ?(@subst_trans OTy _ _) *)
+(*        ?@subst_lift *)
+(*        ?@lift_insert; *)
+(*      try done; *)
+(*      try match goal with *)
+(*        | |- environments.envs_entails _ *)
+(*               (eqₚ ?x ?x) => *)
+(*            iApply eqₚ_intro *)
+(*        | |- environments.envs_entails _ *)
+(*               (eqₚ (insert ?x _ _) (insert ?x _ _)) => *)
+(*            iApply eqₚ_insert; iSplit *)
+(*        end; *)
+(*      auto 1 with typeclass_instances; *)
+(*      try (iStopProof; pred_unfold; *)
+(*           intuition (subst; auto; fail))). *)
+
+(* Ltac wpsimpl := *)
+(*   match goal with *)
+(*   | |- context[fun w : World => prod (?A w) (?B w)] => *)
+(*       change_no_check (fun w : World => prod (A w) (B w)) with (Prod A B) *)
+
+(*   | |- environments.envs_entails _ (bi_impl _ _) => *)
+(*       iIntros "#?" *)
+(*   | |- environments.envs_entails _ (bi_affinely _) => *)
+(*       iModIntro *)
+(*   | |- environments.envs_entails _ (bi_and _ _) => *)
+(*       iSplit *)
+(*   | |- environments.envs_entails _ (eqₚ _ _) => *)
+(*       wpeq *)
+(*   | |- environments.envs_entails _ (bi_pure True) => *)
+(*       done *)
+(*   | |- environments.envs_entails _ (WP (pure _) _) => *)
+(*       rewrite -wp_pure ?trans_refl_r ?trans_refl_r ?subst_refl *)
+(*       (* try (iStopProof; pred_unfold; intuition (subst; auto; fail)) *) *)
+(*   | |- environments.envs_entails _ (WP (bind _ _) _) => *)
+(*       iApply wp_bind *)
+(*   | |- environments.envs_entails _ (WP pick _) => *)
+(*       rewrite -wp_pick; iIntros (?w ?θ) "!>"; iIntros (?τ) "#?" *)
+(*   | |- environments.envs_entails _ (WP (equals _ _) _) => *)
+(*       rewrite -wp_equals; iSplit; *)
+(*       [ iStopProof; pred_unfold; intuition (subst; auto; fail) *)
+(*       | iIntros (?w ?θ) "!>" *)
+(*       ] *)
+(*   | |- environments.envs_entails _ (WP fail _) => *)
+(*       rewrite -wp_fail *)
+
+(*   | |- environments.envs_entails _ (WLP (pure _) _) => *)
+(*       rewrite -wlp_pure ?trans_refl_r ?trans_refl_r ?subst_refl *)
+(*   | |- environments.envs_entails _ (WLP (bind _ _) _) => *)
+(*       rewrite -wlp_bind *)
+(*   | |- environments.envs_entails _ (WLP pick _) => *)
+(*       rewrite -wlp_pick; iIntros (?w ?θ) "!>"; iIntros (?τ) *)
+(*   | |- environments.envs_entails _ (WLP (equals _ _) _) => *)
+(*       rewrite -wlp_equals; iIntros "#?" (?w ?θ) "!>" *)
+(*   | |- environments.envs_entails _ (WLP fail _) => *)
+(*       rewrite -wlp_fail *)
+(*   end. *)
